\documentclass[12pt, letterpaper, twoside]{article}
\usepackage[utf8]{inputenc}

\title{Differential Equations - Midterm Review}
\author{Zachary Chao}
\date{March 27 2018}
 
\begin{document}

\maketitle

\setcounter{section}{1}

\section{First Order Differential Equations}
\subsection{Linear Equations; Method of Integrating Factors}
\subsubsection{$$y'+3y=t+e^{-2t}$$}

\begin{enumerate}
	\item This is already in the form $y'+p(t)y=g(t)$ where $p(t)=3$ and $g(t)=t+e^{-2t}$.
	\item Recall that the integrated factor is defined as $e^{\int p(t)dt}$, therefore our integrated factor is $e^{3t}$.
	\item We now multiply out equation by our integrated factor, rendering us $e^{3t}y'+e^{3t}3y=e^{3t}t+e^{3t}e^{-2t}$.
	\item Reduce the left side by using the inverse chain rule, giving us $e^{3t}y\frac{dy}{dt}=e^{3t}t+e^{t}$.\\
		\textbf{Note} The left side will always reduce to the integrated factor and $y$ as that is the purpose of it.
	\item Multiplpy the equation by dt, $e^{3t}ydy=(e^{3t}t+e^{t})dt$.
	\item Integrating the left side is always simple and is always the integrated factor and $y$ as it is a partial integral, $e^{3t}y=\int e^{3t}t+e^{t}dt$.
	\item Integrate the right side by parts.
		$$\int u\ dv = uv - \int v\ du$$
		
		let $u=t \ dt$ and $dv=e^{3t}$.\\
		$du=1$ and $v=\frac{e^{3t}}{3}$.\\
		

	\item
\end{enumerate}

\end{document}