\documentclass[12pt, letterpaper, twoside]{article}
\usepackage[utf8]{inputenc}
\usepackage{ mathrsfs }


\title{Math 260 Notes}
\author{Zachary Chao}
\date{April 03 2018}
 
\newcommand{\real}{\rm I\!R}
\newcommand{\domain}{\mathscr{D}}
\newcommand{\laplace}{\mathcal{L}}
\usepackage{amsmath}



\begin{document}

\section*{6.2 Solutions of IVT}
Theorem 6.2.1 If f is continuous and f' is piecewise continuous, then
$$\laplace\{f'(t)\}=s \laplace\{f(t)\}-f(0)$$

\subsection*{Proof}
$\laplace\{f'(t)\}=\int_0^\infty e^{-st}f'(t)dt$\\
$u=e^{-st}    dv=f'(t)dt$\\
$du=-se^{-st}    v=f(t)$\\
$=e^{-st}f(t)|_0^\infty+\int_0^\infty se^{-st}f(t)dt$\\
$=\lim_{A\to\infty}[e^{-sA}f(A)]-e^0f(0)=s\int_0^\infty e^{-st}f(t)dt$\\
$=0-f(0+s\laplace\{f\}$\\
$=s\laplace\{f\}-f(0)$\\
$$\laplace\{f''\}=s^2\laplace\{f(t)\}-sf(0)-f'(0)$$

\subsection*{Example 1 - Solve $y''-y'-2y=0, y(0)=1, y'(0)=0$}
Begin by taking the Laplace transform of both sides.\\
$\laplace\{y''-y'-2y\}=\laplace\{0\}$\\
As the Laplace is linear we can simply distribute it to all.\\
$\laplace\{y''\}-\laplace\{y'\}-2\laplace\{y\}=0$\\
$s^2Y(s)-sy(0)-y'(0)-[sY(s)-y(0)]-sY(s)=0$\\
$Y(s)$ is the transform solution we are looking for, which is a function of $t$. $y(0)$ is the solution of the function at 0. The solution we are looking for is y(t). $
\laplace\{y(t)\}=Y(s)$\\
Now algebraically isolate $Y(s)$\\
$s^2Y(s)-s-0-sY(s)+1-sY(s)=0$\\
$Y(s)[s^2-s-2]=s-1$\\
$Y(s)=\frac{s-1}{s^2-s-2}=\frac{s-1}{(s-2)(s+1)}$\\
We have now isolated the transform of our solution, we must untransform it to get our solution. We must now solve by partial fractions.\\
$\frac{s-1}{(s-2)(s+1)}=\frac{A}{s-2} + \frac{B}{s+1}$\\
$s-1 = A(s+1)+B(s-2)$\\
$s-1=As+A+Bs+2B$\\
$s-1=(A+B)s+(A-2B)$\\
$A+B=1$\\
$A-2B=-1$\\
$B=\frac{2}{3}$\\
$A=\frac{1}{3}$\\
$Y(s)=\frac{1}{3}\frac{1}{s-1}+\frac{2}{3}\frac{1}{s+1}$\\
$\laplace^{-1}\{Y(s)\}=\laplace^{-1}\{\frac{1}{3}\frac{1}{s-1}+\frac{2}{3}\frac{1}{s+1}\}$\\
$\laplace^{-1}\{Y(s)\}=\frac{1}{3}\laplace^{-1}\{\frac{1}{s-1}\}+\frac{2}{3}\laplace\{\frac{1}{s+1}\}$\\
You get to the next step by using the table of transforms.\\
$\laplace^{-1}\{Y(s)\}=\frac{1}{3}e^{2t}+\frac{3}{2}e^{-t}$\\

\subsection*{Example - Solve $y''+y=sin2t, y(0)=2, y'(0)=1$}
$\laplace\{y''\}+\laplace\{y\}=\laplace\{sin2t\}$\\
Line 5 in table of transforms.\\
$\laplace\{sinat\}=\frac{a}{s^2+a^2}$\\
$s^2Y(s)-sy(0)-y'(0)+Y(s)=\frac{2}{s^2+4}$\\
$s^2Y(s)-2s-1+Y(s)=\frac{2}{s^2+4}$\\
$Y(s)(s^2+1)=2s+1+\frac{2}{s^2+4}$\\
$Y(s)=\frac{2}{s^2+1}+\frac{1}{s^2+1}+\frac{2}{(s^2+1)(s^2+4)}$\\
Solve by partial fractions.\\
$\frac{2}{(s^2+1)(s^2+4)}=\frac{As+B}{s^2+1}+\frac{Cs+D}{s^2+4}$\\
$2=(As+B)(s^2+4)+(Cs+D)(s^2+1)$\\
ALGEBRA SHIT\\
$A+C=0$\\
$B+D=0$\\
$4A+C=0$\\
$4B+D=2$\\
$A=0, B=\frac{2}{3}, C=0, D=\frac{-2}{3}$\\
$Y(s)=\frac{2s}{s^2+1}+\frac{1}{s^2+1}+\frac{2}{(s^2+1)(s^2+4)}$\\
$Y(s)=\frac{2s}{s^2+1}+\frac{2}{3}\frac{1}{s^2+1}+\frac{2}{3}\frac{1}{s^2+1}-\frac{2}{3}\frac{1}{s^2+4}$\\
$Y(s)=\frac{2s}{s^2+1}+\frac{5}{3}\frac{1}{s^2+1}-\frac{2}{3}\frac{1}{s^2+4}$\\
$\laplace^{-1}\{Y(s)\}=2cost+\frac{5}{3}sint-\frac{1}{3}sin2t$\\

\section*{6.3 Heavyside or Step Functions}
\[
  u_c(t) =
  \begin{cases}
  	0 & \text{, $t < c$} \\
  	1 & \text{, $t \geq c$} \\
  \end{cases}
  c \leq 0
\]

\subsection*{Example 1 : Sketch the graph of $y=h(t)$, where $h(t)=u_\pi(t)-u_{2\pi}(t), t \geq 0$}
\[
  h(t) =
  \begin{cases}
  	0 & \text{, $t < \pi$} \\
  	1 & \text{, $\pi \leq t < 2\pi$} \\
  	0 & \text{, $t \geq 2\pi$} \\
  \end{cases}
\]

\subsection*{The Laplace Transform of $u_c(t)$}
$\laplace\{u_c(t)\}=\int_0^\infty e^{-st}u_c(t) dt$\\
$\laplace\{u_c(t)\}=\int_0^c e^{-st}u_c(t) dt + \int_c^\infty e^{-st}u_c(t) dt$\\
$\laplace\{u_c(t)\}=0 + \int_c^\infty e^{-st} dt$\\
$\laplace\{u_c(t)\}=\frac{e^{-st}}{s}, s>0$\\

\subsection*{Consider the function - }
\[
  y= g(t) =
  \begin{cases}
  	0 & \text{, $t < c$} \\
  	f(t-c) & \text{, $t \geq c$} \\
  \end{cases}
\]

Could instead be written by a unit step function,
$$g(t)=u_c(t)f(t-c)$$

\subsection*{Theorem 6.3.1}
$$\laplace\{u_c(t)f(t-c)\} = e^{-cs} \laplace\{f(t)\} = e^{-cs}F(s)$$

\subsection*{Proof}
$\laplace\{u_c(t)f(t-c)\} = \int_0^\infty e^{-st}u_c(t)f(t-c)dt$\\
We cut out from $0 \to c$ because the integral is 0 there.\\
$\laplace\{u_c(t)f(t-c)\} = \int_c^\infty e^{-st}f(t-c) dt$\\
$\epsilon = t-c$\\
$dt = d\epsilon$\\
$\laplace\{u_c(t)f(t-c)\} = \int_0^\infty e^{-s(\epsilon + c)}f(\epsilon) d\epsilon$\\
$\laplace\{u_c(t)f(t-c)\} = \int_0^\infty e^{-s\epsilon}e^{(-sc)}f(\epsilon) d\epsilon$\\
$\laplace\{u_c(t)f(t-c)\} = e^{-sc} \int_0^\infty e^{-s\epsilon} f(\epsilon) d\epsilon$\\
$\laplace\{u_c(t)f(t-c)\} = e^{-cs} \laplace\{f\}$\\
Line 13 in the transform table.


\subsection*{Example : $f(t)=sint+e_{\frac{\pi}{4}}(t)cos(t-\frac{\pi}{4})$}
$$\laplace\{f\}=\frac{1}{s^2+1}+e^{-\frac{\pi}{4}s}\frac{s}{s^2+1}$$

\subsection*{Example 4 : Find the inverse transform of $F(s) = \frac{1-e^{-2s}}{s^2}$}
$F(s) = \frac{1}{s^2} - \frac{e^{-2s}}{s^2}$\\
$\laplace^{-1}\{F(s)\} = t - u_2(t)(t-2)$\\

\subsection*{Homework}
$6.2 : 1-7odd, 11-15$\\
$6.3 : 1,3,5,7,11,13,15,21$\\
Quiz Thursday








\end{document}



