\documentclass[12pt, letterpaper, twoside]{article}
\usepackage[utf8]{inputenc}
%\usepackage{pgfplots}%


\title{First document}
\author{Zachary Chao}
\date{March 27 2018}
 
\begin{document}

\section*{5.2.5}
Find power series solutions and the first four terms of those solutions $$(1-x)y''+y=0, x_0 = 0$$

Set up our $y'', y'$ and $y$.
$$ y = \sum_{n=0}^{\infty} a_0x^n $$ 
$$ y' = \sum_{n=1}^{\infty} na_0x^{n-1} $$ 
$$ y'' = \sum_{n=2}^{\infty} n(n-1)a_0x^{n-2} $$ 
$$ (1-x) \sum_{n=2}^{\infty} n(n-1)a_0x^{n-2} +  \sum_{n=0}^{\infty} a_0x^n = 0$$
Distribute the (1-x)
$$ \sum_{n=2}^{\infty} n(n-1)a_0x^{n-2} - x\sum_{n=2}^{\infty} n(n-1)a_0x^{n-2} +  \sum_{n=0}^{\infty} a_0x^n = 0 $$
We can distribute the x inside because a series is really a limit,
$$ \sum_{n=0}^{\infty} a_nx^n = \lim_{n\to\infty} x \sum_{i=1}^n a_ix^i$$
Distributing through we get
$$ \sum_{n=0}^{\infty} (n+2)(n+1) a_{n+2} x^n - \sum_{n=0}^{\infty} (n+1)na_{n+1}x^n + \sum_{n=0}^{\infty} a_nx^n = 0$$
Skipping some shit because Im too slow \dots
$$ y = \sum{n=0}^{\infty}a_nx^n = a_0+a_1x+a_2x^2+a_3x^3+a_4x^4 + \dots$$
$$    = a_0 + a_1x - \frac{a_0}{2}x^2 - \frac{a_0+a_1}{6}x^3 - \frac{\frac{a_0}{2}+a_1}{12}x^4 - \frac{\frac{a_0}{3}+\frac{5}{6}a_1}{20}x^5 + \dots$$
$$   y = y_1 + y_2  $$
$$ y_1 = a_0[1 - \frac{1}{2}x^2 - \frac{1}{6}x^3 - \frac{1}{24}x^4 + \dots] $$
$$ y_2 = a_1[x - \frac{1}{6}x^3 - \frac{1}{12}x^4 - \frac{1}{24}x^5 + \dots] $$




\section*{Chapter 6}
\subsection*{Laplace Transform}
Motivation - to deal with discontinous fnctions
The laplace transform $f(t)$, defined in $[0, \infty)$, is given by $f(t) \to F(s)$
$$F(s) = \int_0^{\infty} e^{-st}f(t) \ dt$$
The $e^{-st}$ is what causes the improper integral to converge as it goes to zero quite quickly. 
Note, if it was $e^{-st^2}$, the $t^2$ would go to infinity faster than the it is brought to zero 
so there is an issue of convergence and there are cases where there will not be a Laplace transform.\\
$$\mathcal{L} \{f\} = F$$

\subsection*{ex.5 $let f(t) = e^{at}, t \geq 0$}
$$ \mathcal{L} \{f\} = \int_0^\infty e^{-st}e^{at} \ dt$$
$$ \mathcal{L} \{f\} = \lim_{A\to\infty} \int_0^A e^{(-s+a)t} \ dt $$
$$ \mathcal{L} \{f\} = \lim_{A\to\infty} \int_0^A e^{-(s-a)t} \ dt $$
$$ \mathcal{L} \{f\} = \lim_{A\to\infty} [\frac{-1}{(s-a)}e^{-(s-a)t}|_0^A] $$
$$ \mathcal{L} \{f\} = \lim_{A\to\infty} \{\frac{-1}{(s-a)}[e^{-(s-a)A}-1]\} $$
$$ \mathcal{L} \{f\} = - \frac{1}{(s-a)} \lim_{A\to\infty} [e^{-(s-a)A}-1] $$
$$ \mathcal{L} \{f\} = - \frac{1}{(s-a)} [0-1], s>a $$
$$ \mathcal{L} \{f\} = \frac{1}{(s-a)}, s>a $$



\subsection*{ex : Determine the laplace transform of f(t) = 1}
$$ \mathcal{L} \{f\} = \int_0^\infty e^{-st} 1 \ dt $$
$$ \mathcal{L} \{f\} = \int_0^\infty e^{-st} \ dt $$
$$ \mathcal{L} \{f\} = \lim_{A\to\infty} \int_0^\infty e^{-st} \ dt $$
$$ \mathcal{L} \{f\} = \lim_{A\to\infty} (\frac{-1}{s})e^{-st} |_0^A $$
$$ \mathcal{L} \{f\} = \lim_{A\to\infty} (\frac{-1}{s})[e^{-sA}-1] $$
$$ \mathcal{L} \{f\} = -\frac{1}{s}[0-1] $$
$$ \mathcal{L} \{f\} = \frac{1}{s}, s > 0 $$


$$
f(x) = \left\{
        \begin{array}{ll}
            1 & \quad 0 \leq t < 1 \\
            k & \quad t = 1 \\
	    0 & \quad t > 1
        \end{array}
    \right.
$$





\subsection*{idk some sidenote}
The Laplace transform is a linear operator.
$$ \mathcal{L} \{c_1f_1 + c_2f_2\} = c1 \mathcal{L} \{f_1\} + c_2 \mathcal{L} \{f_2\} $$

\subsection*{Theorm 6.12}
\begin{enumerate}
	\item f is piecewise continous on $[0, \infty)$
	\item $|f(t)| \leq ke^{at}$ for $t \geq m, k, a, m$, constants
\end{enumerate}

$f(t)$ is said to be exponential 

\textbf{Hw 6.1 : 1,5ab,7,11}


pg 317


\end{document}





























